src/lib/util/words_and_bytes.s.dfy
@@ -85,3 +85,4 @@ function ConcatenateSeqs<T>(ss:seq<seq<T>>) : seq<T>
 }
 
 }
+
